Weirdness in BabyIP benchmark.

deps/poulet4/P4ABenchmarks/BabyIPProof.v
@@ -1,21 +1,101 @@
 Require Import Poulet4.P4automata.Examples.ProofHeader.
 Require Import Poulet4.P4automata.Examples.BabyIP.
 
+From Hammer Require Import Tactics.
+
+
+Ltac solve_bisim :=
+  match goal with
+  | |- pre_bisimulation ?a ?wp ?i ?R (?C :: _) _ _ =>
+    extend_bisim a wp i R C;
+    idtac R;
+    idtac C
+  | |- pre_bisimulation ?a ?wp ?i ?R (?C :: _) _ _ =>
+    skip_bisim a wp i R C;
+    idtac R;
+    idtac C
+  | |- pre_bisimulation _ _ _ _ [] _ _ =>
+    apply PreBisimulationClose
+  end.
+
+Ltac give_goal :=
+  match goal with
+  | |- pre_bisimulation ?a ?wp ?i ?R (?C :: _) _ _ =>
+       let H := fresh "H" in
+       assert (H: forall q1 q2 : P4automaton.configuration (P4A.interp a),
+                  interp_crel i R q1 q2 -> interp_conf_rel C q1 q2);
+       idtac; [rewrite filter_entails by (typeclasses eauto);
+        simpl;
+        cbn;
+        unfold interp_conf_rel, interp_conf_state, interp_state_template;
+        simpl;
+        intros [[s1 st1] buf1] [[s2 st2] buf2] Hprem Hl1 Hl2 [Hs1 Hs2] valu;
+        simpl in *
+       |]
+  end.
+
+Notation H := (BabyIP1.header + BabyIP2.header).
+Notation A := BabyIP.aut.
+Notation conf := (P4automaton.configuration (P4A.interp A)).
+Definition r_states :=
+  Eval vm_compute in (Reachability.reachable_states BabyIP.aut 20 BabyIP1.Start BabyIP2.Start).
+
+Ltac extend_bisim' :=
+  match goal with
+  | |- pre_bisimulation ?a ?wp ?i ?R (?C :: _) _ _ =>
+       let H := fresh "H" in
+       assert (H: ~(forall q1 q2 : P4automaton.configuration (P4A.interp a),
+                  interp_crel i R q1 q2 -> interp_conf_rel C q1 q2))
+         by (
+           rewrite filter_entails by (typeclasses eauto);
+           simpl;
+           cbn;
+           unfold interp_conf_rel, interp_conf_state, interp_state_template;
+           simpl;
+           match goal with |- ?G => idtac "admitting" G end; admit
+         );
+         pose (t := wp a C);
+         eapply PreBisimulationExtend with (H0 := right H) (W := t);
+         [ tauto | reflexivity |];
+         compute in t;
+         simpl (_ ++ _);
+         unfold t;
+         clear t;
+         clear H
+  end.
+
+Ltac skip_bisim' :=
+  match goal with
+  | |- pre_bisimulation ?a ?wp ?i ?R (?C :: _) _ _ =>
+       let H := fresh "H" in
+       assert (H: forall q1 q2 : P4automaton.configuration (P4A.interp a),
+                  interp_crel i R q1 q2 -> interp_conf_rel C q1 q2)
+         by (match goal with |- ?G => idtac "admitting" G end; admit);
+       eapply PreBisimulationSkip with (H0:=left H);
+       [ exact I | ];
+       clear H
+  end.
+
 Lemma prebisim_babyip:
   pre_bisimulation BabyIP.aut
-                   (WPSymLeap.wp (H:=_))
-                   (separated _ _ _ _)
+                   (WPSymLeap.wp r_states)
+                   (Reachability.reachable_pair r_states)
                    nil
-                   (mk_init 10 BabyIP.aut BabyIP1.Start BabyIP2.Start)
+                   (mk_init _ _ _ BabyIP.aut 10 BabyIP1.Start BabyIP2.Start)
                    (inl (inl BabyIP1.Start), [], [])
                    (inl (inr BabyIP2.Start), [], []).
 Proof.
   idtac "running babyip bisimulation".
-  set (rel0 := mk_init 10 BabyIP.aut BabyIP1.Start BabyIP2.Start).
+  set (rel0 := (mk_init _ _ _ BabyIP.aut 10 BabyIP1.Start BabyIP2.Start)).
   cbv in rel0.
   subst rel0.
-  time (repeat (time solve_bisim)).
-  cbv in *.
-  intuition (try congruence).
-Time Qed.
+  extend_bisim'.
+  extend_bisim'.
+  extend_bisim'.
+  extend_bisim'.
+  apply PreBisimulationClose.
+  unfold interp_crel, interp_conf_rel, interp_conf_state, interp_state_template.
+  vm_compute.
+  sauto.
+Admitted.
 
